theories/partial/choice/tests.v
@@ -47,6 +47,7 @@ f _ = D
 Definition ret {A B} := fun x => Ret A B (Some x).
 Definition rec {A B} x := fun rest => Rec A B unit (fun _ => x) (fun r => rest (r tt)).
 
+
 (*
 Definition test_function_2 : QTerm -> option QTerm.
   Check runProg.
@@ -66,7 +67,7 @@ Definition test_function_2 : QTerm -> option QTerm :=
                (fun x => rec x (fun res => ret <B `res>))
                (ret <D>)).
 
-Notation "'pmatch' t 'with' | x 'in' pattern => case1 | case2" :=
+(*Notation "'pmatch' t 'with' | x 'in' pattern => case1 | case2" :=
   (Pmatch (fun x => t = pattern) (fun x => case1) case2) (at level 50).
 
 Definition test_function_2' : QTerm -> option QTerm :=
@@ -80,7 +81,7 @@ Proof.
   unfold test_function_2', rec, ret.
   evaluate_function solve_all.
   reflexivity.
-Qed.
+Qed.*)
 
 Theorem something_bad : test_function_1 <C> = <B>.
 Proof.
@@ -88,3 +89,101 @@ Proof.
   evaluate_function solve_all.
   easy.
 Qed.  
+
+(* now, test Pmatch2 *)
+
+(*
+f (A x y) = (x, y)
+f _ _ = (D, E)
+ *)
+Check Pmatch.
+Check Pmatch2.
+
+Definition test_function_3 (t : QTerm) : QTerm * QTerm :=
+  Pmatch2 (fun x y => t = <A `x `y>) (fun x y => (x, y)) (<D>, <E>).
+
+Theorem run_test_function_3_1 : test_function_3 <A B C> = (<B>, <C>).
+Proof.
+  unfold test_function_3.
+  evaluate_function solve_all.
+  reflexivity.
+Qed.
+
+Theorem run_test_function_3_2 : test_function_3 <C> = (<D>, <E>).
+Proof.
+  unfold test_function_3.
+  evaluate_function solve_all.
+  reflexivity.
+Qed.
+
+(*
+Ok, now a function which uses both Pmatch2 and general recursion
+f (A x y) = B (f x) (f y)
+f _ = D
+ *)
+
+Check Rec.
+Definition test_function_4 : QTerm -> option QTerm.
+  refine (
+      runProg (fun t =>
+             Pmatch2
+               (fun x y => t = <A `x `y>)
+               (fun x y => Rec _ _ bool
+                               (fun b => if b then x else y)
+                               (fun rec => ret <B {rec true} {rec false}>)
+               )
+               (ret <D>))
+
+    ).
+Defined.
+
+Theorem run_test_function_4_1 : test_function_4 <A E F> = Some <B D D>.
+Proof.
+  unfold test_function_4.
+  evaluate_function solve_all.
+  (* SO, this demonstrates the problem! *)
+  Fail Qed.
+Abort.
+
+
+(* a simpler demonstration of the problem: 
+
+again,
+f (A x) = B (f x)
+f _ = D
+
+
+but this time write the definition so it can't beta-normalize away the index family when
+applied to a free variable
+
+*)
+
+
+Definition test_function_5 : QTerm -> option QTerm :=
+  runProg (fun t =>
+             Pmatch
+               (fun x => t = <A `x>)
+               (fun x => Rec _ _ unit
+                             (fun u => match u with tt => x end)
+                             (fun res => ret <B {res tt}>))
+               (ret <D>)).
+
+Theorem run_test_function_5_1 : test_function_5 <A (A C)> = Some <B (B D)>.
+Proof.
+  unfold test_function_5.
+  evaluate_function solve_all.
+  Check runProgDefinitionRec.
+  Check PmatchDef1.
+  Check @Pmatch.
+  Locate "with".
+  Set Printing All.
+  Check Pmatch.
+  Fail reflexivity.
+Abort.
+
+(*
+one idea is that if i have a default case for the function, then
+i don't need the option.
+then i also wouldn't need collectOption.
+i'll try this in prog3
+*)
