theories/metaprogramming/patternMatchingTest.v
@@ -1,0 +1,85 @@
+Require Import String.
+Require Import qterm.
+Require Import lambdaFacts.
+Require Import lambdaSolve.
+Require Import FunctionalExtensionality.
+Require Import Coq.Logic.PropExtensionality.
+
+(*
+the goal of this file is to test if pattern matching works.
+i know already that there will be a transport hell issue.
+instead, i'm going to try to prove something by pattern matching that shouldn't
+get stuck on that
+
+TODO: what thing, maybe pulling a body from a lambda? is that already in substitution.v?
+
+*)
+
+Definition pair := <fun t1 => fun t2 => fun p => p t1 t2>.
+Notation "t1 , t2" := <`pair `t1 `t2> (in custom term_term at level 30,
+                                       t1 custom term_term,
+                                             t2 custom term_term) : term_scope.
+
+Notation "'proj1' t" := <`t (fun x => fun y => x)> (in custom term_term at level 35,
+                                  t custom term_term, only parsing) : term_scope.
+Notation "'proj2' t" := <`t (fun x => fun y => y)> (in custom term_term at level 35,
+                                  t custom term_term, only parsing) : term_scope.
+
+(* Contexts *)
+Definition nil := <Nil>.
+Definition cons := <fun ctx => fun lvl => fun ty => Cons ctx lvl ty>.
+
+(* Variables *) 
+Definition zero := <fun env => proj2 env>.
+Definition succ := <fun x => fun env => x (proj1 env)>.
+
+Definition pi := <fun x => fun y => fun env => Pi (x env) (fun a => y (env , a))>.
+Definition U : QTerm := <fun env => U>.
+Definition Empty := <fun env => Empty>.
+Definition Bool := <fun env => Bool>.
+Definition Lift := <fun T => fun env => Lift (T env)>.
+
+Definition var_to_term := <fun x => x>.
+Definition lambda := <fun t => fun env => fun a => t (env , a)>.
+Definition app := <fun t1 => fun t2 => fun env => (t1 env) (t2 env)>.
+Definition true := <fun env => fun p => proj1 p>.
+Definition false := <fun env => fun p => proj2 p>.
+Definition ifexpr := <fun cond => fun t1 => fun t2 => fun env => (cond env) (t1 env , t2 env)>.
+
+Definition weaken := <fun t => fun env => t (proj1 env)>.
+Definition subLast := <fun t => fun toSub => fun env => t (env , (toSub env))>.
+
+Ltac unfold_all := unfold nil, cons, zero, succ, pi, U, Bool, Empty, var_to_term, lambda,
+    app, weaken, subLast, true, false, ifexpr, Lift, pair in *.
+
+(* The deeper shallow embedding *)
+
+Inductive VarTyped : QTerm -> nat -> QTerm -> QTerm -> Prop :=
+| ty_zero : forall ctx T lvl, VarTyped <`cons `ctx {const (term.nconst lvl)} `T> lvl <`weaken `T> zero
+| ty_succ : forall ctx A T s lvl1 lvl2, VarTyped ctx lvl1 A s
+                              -> VarTyped <`cons `ctx `lvl2 `T> lvl1 <`weaken `A> <`succ `s>.
+
+Inductive Typed : (*context*) QTerm -> (*level*) nat -> (*Type*) QTerm -> (*Term*) QTerm -> Prop :=
+| ty_lambda : forall ctx A B s lvl,
+    Typed ctx (S lvl) <`U> <`pi `A `B> ->
+    Typed <`cons `ctx {const (term.nconst lvl)} `A> lvl B s -> Typed ctx lvl <`pi `A `B> <`lambda `s>
+| ty_app : forall ctx A B s1 s2 lvl, Typed ctx lvl <`pi `A `B> s1 -> Typed ctx lvl A s2
+                                 -> Typed ctx lvl <`subLast `B `s2> <`app `s1 `s2>
+| ty_var : forall ctx T t lvl, VarTyped ctx lvl T t -> Typed ctx lvl T t
+| ty_true : forall ctx, Typed ctx 0 Bool true
+| ty_false : forall ctx, Typed ctx 0 Bool false
+| ty_if : forall ctx T cond t1 t2 lvl,
+    Typed ctx lvl Bool cond ->
+    Typed ctx lvl <`subLast `T `true> t1 ->
+    Typed ctx lvl <`subLast `T `false> t2 ->
+    Typed ctx lvl <`subLast `T `cond> <`ifexpr `cond `t1 `t2>
+| ty_Empty : forall ctx, Typed ctx 1 <`U> Empty
+| ty_Bool : forall ctx, Typed ctx 1 <`U> Bool
+| ty_pi : forall ctx A B lvl,
+    Typed ctx (S lvl) <`U> A
+    -> Typed <`cons `ctx {const (term.nconst lvl)} `A> (S lvl) <`U> B -> Typed ctx (S lvl) <`U> <`pi `A `B>
+| ty_U : forall ctx lvl, Typed ctx (S (S lvl)) <`U> <`U>
+| ty_Lift : forall ctx lvl T, Typed ctx (S lvl) <`U> T -> Typed ctx (S (S lvl)) <`U> <`Lift `T>
+| ty_lift : forall ctx lvl T t, Typed ctx lvl T t -> Typed ctx (S lvl) <`Lift `T> t
+| ty_lower : forall ctx lvl T t, Typed ctx (S lvl) <`Lift `T> t -> Typed ctx lvl T t
+.
