theories/metaprogramming/typechecking.v
@@ -1,0 +1,144 @@
+Require Import String.
+Require Import qterm.
+Require Import lambdaFacts.
+Require Import lambdaSolve.
+Require Import FunctionalExtensionality.
+Require Import Coq.Logic.PropExtensionality.
+
+(*
+in this file, i'm making sure that typechecking will work.
+the idea is that i can build up a term out of the constructors of the deep embedding,
+and put casts in between when they don't directly line up.
+then solve_all at the end.
+the question is does this work out.
+
+also, i need to find out what term to test this on, but for now just the simplest one.
+ *)
+
+Definition pair := <fun t1 => fun t2 => fun p => p t1 t2>.
+Notation "t1 , t2" := <`pair `t1 `t2> (in custom term_term at level 30,
+                                       t1 custom term_term,
+                                             t2 custom term_term) : term_scope.
+
+Notation "'proj1' t" := <`t (fun x => fun y => x)> (in custom term_term at level 35,
+                                  t custom term_term, only parsing) : term_scope.
+Notation "'proj2' t" := <`t (fun x => fun y => y)> (in custom term_term at level 35,
+                                  t custom term_term, only parsing) : term_scope.
+
+Module S.
+  Definition nil := <Nil>.
+  Definition cons := <fun ctx => fun lvl => fun ty => Cons ctx lvl ty>.
+
+  Definition zero := <fun env => proj2 env>.
+  Definition succ := <fun x => fun env => x (proj1 env)>.
+
+  Definition pi := <fun x => fun y => fun env => Pi (x env) (fun a => y (env , a))>.
+  Definition U : QTerm := <fun env => U>.
+  Definition Empty := <fun env => Empty>.
+  Definition Bool := <fun env => Bool>.
+  Definition Lift := <fun T => fun env => Lift (T env)>.
+
+  Definition var_to_term := <fun x => x>.
+  Definition lambda := <fun t => fun env => fun a => t (env , a)>.
+  Definition app := <fun t1 => fun t2 => fun env => (t1 env) (t2 env)>.
+  Definition true := <fun env => fun p => proj1 p>.
+  Definition false := <fun env => fun p => proj2 p>.
+  Definition ifexpr := <fun cond => fun t1 => fun t2 => fun env => (cond env) (t1 env, t2 env)>.
+
+  Definition weaken := <fun t => fun env => t (proj1 env)>.
+  Definition subLast := <fun t => fun toSub => fun env => t (env , toSub env)>.
+
+  (* Shallow substitutions *)
+  Definition idSub := <fun env => env>. (* : Sub ctx ctx *)
+  Definition weaken1Ren := <fun env => proj1 env>. (* : Sub ctx (ctx, T) *)
+  (* liftSub : Sub ctx1 ctx2 -> Sub (cons ctx1 lvl T) (cons ctx2 lvl (subTerm sub T)) *)
+  Definition liftSub := <fun sub => fun env => (sub (proj1 env), proj2 env)>.
+  (* subTerm : (sub : Sub ctx1 ctx2) -> Term ctx1 T -> Term ctx2 (subTerm sub T) *)
+  (* extendSub : Sub ctx1 ctx2 -> Term ctx1 T -> Sub (ctx1, T) ctx2 *)
+  Definition extendSub := <fun sub => fun t => fun env => (sub env, t (sub env))>.
+  Definition subTerm := <fun sub => fun t => fun env => t (sub env)>.
+
+  Ltac unfold_all := unfold nil, cons, zero, succ, pi, U, Bool, Empty, var_to_term, lambda,
+      app, weaken, subLast, true, false, ifexpr, Lift,
+      idSub, weaken1Ren, liftSub, subTerm, pair in *.
+End S.
+
+(* The deeper shallow embedding *)
+
+Inductive Var : QTerm -> nat -> QTerm -> QTerm -> Type :=
+| zero : forall {ctx T lvl}, Var <`S.cons `ctx {const (term.nconst lvl)} `T> lvl <`S.weaken `T> S.zero
+| succ : forall {ctx A T s lvl1 lvl2}, Var ctx lvl1 A s
+                              -> Var <`S.cons `ctx `lvl2 `T> lvl1 <`S.weaken `A> <`S.succ `s>.
+
+Inductive Typed : (*context*) QTerm -> (*level*) nat -> (*Type*) QTerm -> (*Term*) QTerm -> Type :=
+| lambda : forall {ctx A B s lvl},
+    (*Typed ctx (S lvl) <`U(*{const lvl}*)> <`pi `A `B> ->*)
+    Typed <`S.cons `ctx {const (term.nconst lvl)} `A> lvl B s -> Typed ctx lvl <`S.pi `A `B> <`S.lambda `s>
+| app : forall {ctx A B s1 s2 lvl}, Typed ctx lvl <`S.pi `A `B> s1 -> Typed ctx lvl A s2
+                                  -> Typed ctx lvl <`S.subLast `B `s2> <`S.app `s1 `s2>
+| ann_app : forall ctx A B s1 s2 lvl,
+    Typed ctx (S lvl) S.U A
+    -> Typed ctx lvl <`S.pi `A `B> s1 -> Typed ctx lvl A s2
+    -> Typed ctx lvl <`S.subLast `B `s2> <`S.app `s1 `s2>
+| var : forall {ctx T t lvl}, Var ctx lvl T t -> Typed ctx lvl T t
+| true : forall {ctx}, Typed ctx 0 S.Bool S.true
+| false : forall {ctx}, Typed ctx 0 S.Bool S.false
+(*
+| if : forall ctx T cond t1 t2 lvl,
+    Typed ctx lvl Bool cond ->
+    Typed ctx lvl <`subLast `T `true> t1 ->
+    Typed ctx lvl <`subLast `T `false> t2 ->
+    Typed ctx lvl <`subLast `T `cond> <`ifexpr `cond `t1 `t2>
+| Empty : forall ctx, Typed ctx 1 <`U(*{const 0}*)> Empty
+| Bool : forall ctx, Typed ctx 1 <`U(*{const 0}*)> Bool
+| pi : forall ctx A B lvl,
+    Typed ctx (S lvl) <`U(*{const lvl}*)> A
+    (* TODO: is S lvl correct below? *)
+    -> Typed <`cons `ctx {const lvl} `A> (S lvl) <`U(*{const lvl}*)> B -> Typed ctx (S lvl) <`U(*{const lvl}*)> <`pi `A `B>
+| U : forall ctx lvl, Typed ctx (S (S lvl)) <`U(*{const (S lvl)}*)> <`U(*{const lvl}*)>
+| Lift : forall ctx lvl T, Typed ctx (S lvl) <`U> T -> Typed ctx (S (S lvl)) <`U> <`Lift `T>
+| lift : forall ctx lvl T t, Typed ctx lvl T t -> Typed ctx (S lvl) <`Lift `T> t
+| lower : forall ctx lvl T t, Typed ctx (S lvl) <`Lift `T> t -> Typed ctx lvl T t
+*)
+.
+
+Ltac solve_no_unfold := repeat (lambda_solve ; repeat neutral_inj_case ;lambda_solve
+                  ; repeat fast_neutral_unequal_case). 
+
+Ltac solve_all := repeat (S.unfold_all ; lambda_solve ; (repeat neutral_inj_case ;lambda_solve)
+                          ; (repeat fast_neutral_unequal_case); (repeat simple_pattern_case);
+                          hide_evars;
+                          rewrite <- ?eta;
+                          sort_lifts;
+                          unhide_evars).
+
+
+Definition cast {ctx1 ctx2 lvl1 lvl2 ty1 ty2 tm1 tm2}
+           {_ : ctx1 = ctx2}
+           {_ : lvl1 = lvl2}
+           {_ : ty1 = ty2}
+           {_ : tm1 = tm2}
+           (prog : Typed ctx1 lvl1 ty1 tm1) : Typed ctx2 lvl2 ty2 tm2.
+  subst.
+  apply prog.
+Defined.
+
+Definition castVar {ctx1 ctx2 lvl1 lvl2 ty1 ty2 tm1 tm2}
+           {_ : ctx1 = ctx2}
+           {_ : lvl1 = lvl2}
+           {_ : ty1 = ty2}
+           {_ : tm1 = tm2}
+           (prog : Var ctx1 lvl1 ty1 tm1) : Var ctx2 lvl2 ty2 tm2.
+  subst.
+  apply prog.
+Defined.
+
+
+
+(*
+the term should be
+((fun x : Bool => x) true) : Bool
+*)
+Definition test_typecheck_1 : Typed S.nil 0 S.Bool S.true.
+  refine (cast (app (lambda (var zero)) true)); solve_all.
+Defined.
