theories/partial/choice/prog3.v
@@ -1,0 +1,192 @@
+Require Import Classical.
+Require Import FunctionalExtensionality.
+Require Import Coq.Logic.PropExtensionality.
+
+Require Import choiceBase.
+
+(*
+in this file, i'm doing a version that uses a default value so there doesn't need to be
+and option monad. i'm hoping this will make things way simpler.
+*)
+Inductive Prog (A B : Type) : Type :=
+| Ret : B -> Prog A B
+| Rec : forall (I : Type) (args : I -> A), ((I -> B) -> Prog A B) -> Prog A B
+.
+
+Inductive runProgR {A B : Type} (def : A -> Prog A B) : Prog A B -> B -> Prop :=
+| retR : forall b, runProgR def (Ret _ _ b) b
+| recR : forall I
+                (args : I -> A)
+                (recVals : I -> B)
+                (res : B)
+                (rest : (I -> B) -> Prog A B),
+    (* if for all inputs a satisfying P, recVals describes the recursive calls *)
+    (forall (i : I), runProgR def (def (args i)) (recVals i))
+    (* and given the results of those recursive calls, the program outputs res *)
+    -> runProgR def (rest recVals) res
+    (* then overall res *)
+    -> runProgR def (Rec _ _ I args rest) res
+.
+
+Theorem runProgFunction {A B : Type} {def : A -> Prog A B} {p : Prog A B} {b1 b2 : B}
+  (rp1 : runProgR def p b1) (rp2 : runProgR def p b2) : b1 = b2.
+Proof.
+  intros.
+  generalize rp2.
+  generalize b2.
+  clear rp2.
+  clear b2.
+  induction rp1.
+  - intros.
+    inversion rp2.
+    reflexivity.
+  - intros.
+    inversion rp2.
+    apply exist_inj2_uip in H2.
+    subst.
+    apply IHrp1.
+    assert (rest1 = rest). {
+      apply exist_inj2_uip in H4.
+      assumption.
+    }
+    subst.
+    assert (recVals = recVals0). {
+      extensionality i.
+      specialize (H i).
+      specialize (H5 i).
+      apply H0.
+      apply H5.
+    }
+    subst.
+    assumption.
+Qed.
+
+Definition chooseDefault (T : Type) (P : T -> Prop) (default : T) : T.
+  refine (choose T (fun t => P t \/ ((~exists t, P t) /\ t = default))).
+  destruct (classic (exists t, P t)).
+  - destruct H.
+    exists x.
+    apply or_introl.
+    assumption.
+  - exists default.
+    apply or_intror.
+    easy.
+Defined.
+
+Definition runProgImpl {A B : Type} (def : A -> Prog A B) (p : Prog A B) (default : B) : B.
+  refine (chooseDefault B (fun b => runProgR def p b) default).
+Defined.
+
+Definition runProg {A B : Type} (def : A -> Prog A B) (a : A) (default : B) : B :=
+  (runProgImpl def (def a) default).
+
+Theorem runProgDefinitionRet {A B : Type} (def : A -> Prog A B) (b : B) default
+  : runProgImpl def (Ret _ _ b) default = b.
+  unfold runProgImpl, chooseDefault.
+  apply choiceInd.
+  intros.
+  destruct H.
+  - inversion H.
+    subst.
+    reflexivity.
+  - destruct H.
+    subst.
+    exfalso.
+    apply H.
+    exists b.
+    constructor.
+Qed.
+
+(*
+can't i simplify things way further here?
+do i even need the Prog datatype at all if i have this default concept?
+
+like,
+
+runProg : (default : B) -> ((reccall : A -> B) -> A -> B) -> A -> B
+
+the reason why you can't normally define general recursion by a fixpoint is becuase with
+
+runProg : ((reccall : A -> option B) -> A -> option B) -> A -> option B
+
+there is nothing to stop it from doing something like checking if the recursive call outputs
+Some or None, which doesn't make sense for a recursive function.
+
+
+
+does this work?
+
+runProg d f a = f (runProg d f)
+
+
+
+before any of that, does my original idea for this file even work?
+
+*)
+
+Theorem runProgDefinitionRec {A B : Type} {def : A -> Prog A B}
+        {I : Type}
+        {args : I -> A}
+        {rest : (I -> B) -> Prog A B}
+        {default}
+  : runProgImpl def (Rec _ _ I args rest) default =
+           runProgImpl def (rest (fun i => runProg def (args i) default)) default.
+Proof.
+  repeat unfold runProgImpl, runProg, chooseDefault.
+  repeat apply choiceInd.
+  intros.
+  destruct H.
+  - inversion H.
+    
+    
+Qed.    
+
+
+(*
+As an example to test recursion with infinite recursive calls per call,
+take the function
+f : nat * nat -> Prop
+f (0, _) = True
+f (S n, _) = not (forall m, f (n, m))
+
+The goal is to see if I can automate the running of this function.
+The output should not just be True or False, but should be a proposition expression built out
+of the recurrence.
+ *)
+Check Rec.
+
+Definition fImpl : nat * nat -> Prog (nat * nat) Prop :=
+  fun nm => match nm with
+            | (O, _) => Ret _ _ (Some True)
+            | (S n, m) => Rec _ _ _
+                                  (fun (i : nat) => (n, i))
+                                         (fun rec => Ret _ _ (Some
+                                 (not (forall m, rec m))))
+            end.
+
+Definition exampleInfFun : nat * nat -> option Prop.
+  refine (runProg fImpl).
+Defined.
+
+(* Now to try to run the function: *)
+Theorem runExampleFun : exampleInfFun (1, 5) = Some False.
+
+  repeat (try unfold exampleInfFun, runProg;
+          try rewrite runProgDefinitionRet;
+          try rewrite runProgDefinitionRec;
+          try rewrite collectOptionDef;
+          simpl).
+
+  assert ((~ (nat -> True)) = False). {
+    apply propositional_extensionality.
+    split.
+    - intros.
+      apply H.
+      auto.
+    - intros.
+      exfalso.
+      assumption.
+  }
+  rewrite H.
+  reflexivity.
+Qed.
