theories/partial/choice/prog4.v
@@ -1,0 +1,96 @@
+Require Import Classical.
+Require Import FunctionalExtensionality.
+Require Import Coq.Logic.PropExtensionality.
+
+Require Import choiceBase.
+
+(*
+in this file, i'm tyring a version where you can just directly write a function in terms
+of a recursive thing.
+*)
+
+Inductive runProgR {A B : Type} (prog : (A -> B) -> A -> B) : A -> B -> Prop :=
+| c :forall (S : A -> Prop) a b (par : A -> B),
+    (forall a' b', S a' -> par a' = b' -> runProgR prog a' b')
+    -> (forall (f : A -> B), (forall a, S a -> par a = (f a)) -> prog f a = b)
+    -> runProgR prog a b
+.
+
+Theorem runProgFunction {A B : Type} {a : A} {prog : (A -> B) -> A -> B} {b1 b2 : B}
+  (rp1 : runProgR prog a b1) (rp2 : runProgR prog a b2) : b1 = b2.
+Proof.
+  intros.
+  generalize rp2.
+  generalize b2.
+  clear rp2.
+  clear b2.
+  induction rp1.
+  intros.
+  inversion rp2.
+  subst.
+  (* idea:
+       - show that par and par0 correspond on intersection of S and S0
+       - find f : A -> B that is the union of par and par0 (using choice)
+       - show that both b and b2 are equal to prog f a for this f, using H1 and H3.
+   *)
+  assert (forall a, S a -> S0 a -> par a = par0 a) as paragree. {
+    intros.
+    specialize (H2 a0 (par0 a0) H5 eq_refl).
+    specialize (H0 a0 (par a0) H4 eq_refl (par0 a0) H2).
+    assumption.
+  }
+  pose (f := fun a => Pif (S a) (par a) (Pif (S0 a) (par0 a) b)).
+  assert (forall a, S a -> par a = f a) as fAgreesPar. {
+    intros.
+    unfold f.
+    rewrite (PifDef1 _ _ _ _ H4).
+    reflexivity.
+  }
+  assert (forall a, S0 a -> par0 a = f a) as fAgreesPar0. {
+    intros.
+    destruct (classic (S a0)).
+    - rewrite <- paragree; auto.
+    - unfold f.
+      rewrite (PifDef2 _ _ _ _ H5).
+      rewrite (PifDef1 _ _ _ _ H4).
+      reflexivity.
+  }
+  specialize (H1 f fAgreesPar).
+  specialize (H3 f fAgreesPar0).
+  rewrite <- H1, H3.
+  reflexivity.
+Qed.
+
+Definition chooseDefault (T : Type) (P : T -> Prop) (default : T) : T.
+  refine (choose T (fun t => P t \/ ((~exists t, P t) /\ t = default))).
+  destruct (classic (exists t, P t)).
+  - destruct H.
+    exists x.
+    apply or_introl.
+    assumption.
+  - exists default.
+    apply or_intror.
+    easy.
+Defined.
+
+Definition runProg {A B : Type} (prog : (A -> B) -> A -> B) (default : B) (a : A) : B.
+  refine (chooseDefault B (fun b => runProgR prog a b) default).
+Defined.
+
+Theorem runProgDef {A B : Type} (prog : (A -> B) -> A -> B) (default : B) (a : A) 
+  : runProg prog default a = prog (runProg prog default) a.
+Proof.
+
+  (*
+    i don't this that this works as is.
+    suppose that there is abad : A, such that (runProg prog d abad = d)
+    then suppose that (prog f a' = 1 + abad).
+    then (runProg prog d a' = default),
+    but actually this theorm wants it to be (1 + default).
+
+    i thiink that i can fix this by adjusting the definition of runProgR,
+    basically make it include the defaults itself and be total.
+    add a second constructor that inputs the negation of the premises of the first constructor
+    and then says it outputs a default there.
+    using lem, this will trivially be total.
+*)
